ACL2Lean/DSL.lean
@@ -76,6 +76,11 @@ def mapBuiltinStx (s : String) : Ident :=
     | "append" => `_root_.ACL2.Logic.append
     | "len" => `_root_.ACL2.Logic.len
     | "true-listp" => `_root_.ACL2.Logic.trueListp
+    | "iff" => `_root_.ACL2.Logic.iff
+    | "force" => `_root_.ACL2.Logic.force
+    | "double-rewrite" => `_root_.ACL2.Logic.double_rewrite
+    | "evens" => `_root_.ACL2.Logic.evens
+    | "odds" => `_root_.ACL2.Logic.odds
     | s' => sanitize s'
   mkIdent name
 
@@ -123,7 +128,7 @@ partial def translateSExprValue (stx : Syntax) : MacroM (TSyntax `term) := do
 
 /-- Detect built-ins to avoid collecting them as variables. -/
 def isBuiltin (s : String) : Bool :=
-  ["+", "-", "*", "/", "<", ">", "=", "<=", ">=", "if", "zp", "evenp", "equal", "consp", "atom", "car", "cdr", "cons", "not", "and", "or", "implies", "t", "nil", "quote", "let", "declare", "stringp", "string-append", "logand", "logor", "logxor", "lognot", "ash", "append", "len", "true-listp"].contains s
+  ["+", "-", "*", "/", "<", ">", "=", "<=", ">=", "if", "zp", "evenp", "equal", "consp", "atom", "car", "cdr", "cons", "not", "and", "or", "implies", "t", "nil", "quote", "let", "declare", "stringp", "string-append", "logand", "logor", "logxor", "lognot", "ash", "append", "len", "true-listp", "iff", "force", "double-rewrite", "evens", "odds"].contains s
 
 /-- Collect free variables. -/
 partial def collectFreeVars (stx : Syntax) : MacroM (List Ident) := do
